program_logic/WhileCycle.ec
@@ -1,12 +1,14 @@
 pragma Goals:printall.
 require import Int.
 
-type rrt, irt, sbits.
+type rrt, irt, sbits, dt, de.
 
 op MyPred : rrt -> bool.
 
+op df : irt -> rrt -> de -> dt.
+
 module type Dist = {
-  proc run(r:rrt) : bool
+  proc guess(r:dt) : bool
 }.
 
 
@@ -26,17 +28,20 @@ import IM.
 
 require PrIntervalToSum.
 clone import PrIntervalToSum as PIT with type rt <- bool * rrt,
-                                            type iat <- (rrt -> bool) * irt * int * int * rrt .
+                                            type iat <- ((rrt -> bool) * irt * int * int * rrt)*de .
 
 section.
 
 declare module A <: Run {-W, -DW}.
-declare module D <: Dist {-A, -W, -DW}.
+declare module D <: Dist {-W, -DW}.
 
 declare axiom A_ll : islossless A.run.
 declare axiom A_rew_ph x : phoare[ A.run : (glob A) = x ==> !MyPred res => (glob A) = x ] = 1%r.
+axiom A_rew_hoare x : hoare[ A.run : (glob A) = x ==> !MyPred res => (glob A) = x ] .
 
-declare axiom D_ll : islossless D.run.
+declare axiom whp_axp : equiv[ D.guess ~ D.guess : ={glob A, arg} ==> ={res}  ].
+
+declare axiom D_ll : islossless D.guess.
 
 lemma if_whp_prop : 
   equiv [ W(A).whp ~ W(A).if_whp : ={glob W, glob A, arg} ==>  ={glob W, glob A, res} ].
@@ -103,21 +108,22 @@ skip. progress.
 qed.
 
 
-local module W0 = {
-  proc run(a : irt ) = {
+
+module W0(A : Run, D : Dist) = {
+  proc run(a : irt,w:de) = {
       var r, b;
       r <@ A.run(a);
-      b <@ D.run(r);
+      b <@ D.guess(df a r w);
       return (b, r);
   }
 }.
 
-local module W1 = {
+module W1(A : Run, D : Dist) = {
   module M = W(A)
-  proc run(a : (rrt -> bool) * irt * int * int * rrt ) = {
+  proc run(a : (rrt -> bool) * irt * int * int * rrt, w: de) = {
       var r, b;
       r <@ M.whp(a);
-      b <@ D.run(r);
+      b <@ D.guess(df a.`2 r w);
       return (b, r);
   }
 }.
@@ -125,38 +131,76 @@ local module W1 = {
 
 local module W2 = {
   module M = W(A)
-  proc run(a : (rrt -> bool) * irt * int * int * int * rrt ) = {
+  proc run(a : (rrt -> bool) * irt * int * int * int * rrt, w:de ) = {
       var r, b;
       r <@ M.whp_split(a);
-      b <@ D.run(r);
+      b <@ D.guess(df a.`2 r w);
       return (b, r);
   }
 }.
 
 local module W3 = {
   module M = W(A)
-  proc run(a : (rrt -> bool) * irt * int * int * rrt ) = {
+  proc run(a : (rrt -> bool) * irt * int * int * rrt,w:de ) = {
       var r, b;
       r <@ M.whp_if(a);
-      b <@ D.run(r);
+      b <@ D.guess(df a.`2 r w);
       return (b, r);
   }
 }.
 
+print W.
+
+
+
+local module W3' = {
+  module M = W(A)
+  proc run(a : (rrt -> bool) * irt * int * int * rrt,w:de ) = {
+    var r, b,ri;   
+    ri <@ M.whp(a.`1, a.`2, a.`3, a.`4-1, a.`5);
+    if (W.c <= a.`4 /\ ! a.`1 ri) {
+      W.c <- W.c+1;
+      (b,r) <@ W0(A,D).run(a.`2,w);
+    }else{
+      r <- ri;
+      b <@ D.guess(df a.`2 r w);
+    }
+    return (b, r);
+  }
+}.
+
+
+local lemma w3w3' : equiv[ W3.run ~ W3'.run : ={arg, glob A, glob W} ==> ={res, glob W} ].
+proof. proc.
+inline W3.M.whp_if. sp.  elim*. progress.
+seq 1 1 : ( ={w,a,ri, glob A, glob W} /\ p{1} = a.`1{2} /\ e{1} = a.`4{2} /\ i{1} = a.`2{2} ). 
+inline*. sp. 
+wp. 
+while (={a,  w, glob A, glob W} /\ p{1} = a{2}.`1 /\ i{1} = a.`2{2} /\  i0{1} = i{2} /\ e0{1} = e{2} /\ p0{1} = p{2} /\ r1{1} = r0{2} /\ e{1} = a.`4{2}).
+wp.  call (_:true). skip. progress. skip. progress.
+
+if. smt.
+inline*. wp.  sp.  call whp_axp. wp.  call (_:true). skip. progress. 
+call whp_axp. wp.  skip. progress. 
+qed.
+
+
+
+
 
 local module W4 = {
   module M = W(A)
-  proc run(a : (rrt -> bool) * irt * int * int * rrt ) = {
+  proc run(a : (rrt -> bool) * irt * int * int * rrt,w:de ) = {
       var r;
       M.whp(a);
-      r <@ W0.run(a.`2);
+      r <@ W0(A,D).run(a.`2,w);
       return r;
   }
 }.
 
 local lemma whp_premat_1_eq  pa ia sa ea ra ja : sa <= ja => ja <= ea + 1 =>
   equiv [ W(A).whp ~  W(A).whp_split : arg{1} = (pa,ia,sa,ja-1,ra) 
-  /\ arg{2} = (pa,ia,sa,ja-1,ea,ra) /\  ={glob A} ==>  ((W.c = ja /\ pa res){1} /\ (W.c = ja /\ pa res){2} => ={res})    /\ (W.c = ja /\ pa res){1}  <=> (W.c = ja /\ pa res){2}  ].
+  /\ arg{2} = (pa,ia,sa,ja-1,ea,ra) /\  ={glob A} ==>   (((W.c = ja /\ pa res){1} /\ (W.c = ja /\ pa res){2} => ={res, glob A})    /\ (W.c = ja /\ pa res){1}  <=> (W.c = ja /\ pa res){2} )  ].
 proof. move => hp ph.
 proc*.
 inline W(A).whp_split. sp.
@@ -168,10 +212,10 @@ inline*.  sp.
 case (pa r0{1}).
 rcondf {2} 1. progress.  skip. progress. smt.
 wp. skip. progress. wp.
-conseq (_:  (p1{2} = pa /\ r2{2} = r0{1}) /\ ja  -1 <= e0{2}  /\  (! pa r0{1}) /\ W.c{1} = ja  /\ W.c{2} = W.c{1} /\ e1{2} = e0{2} /\ e1{2} = ea  ==> _ ). progress. smt.  smt.
+conseq (_:  ={glob A} /\(p1{2} = pa /\ r2{2} = r0{1}) /\ ja  -1 <= e0{2}  /\  (! pa r0{1}) /\ W.c{1} = ja  /\ W.c{2} = W.c{1} /\ e1{2} = e0{2} /\ e1{2} = ea  ==> _ ). progress. smt.  smt.
 case ((W.c <= e1 /\ ! p1 r2){2}).
 unroll {2} 1. rcondt{2} 1. progress.
-seq 0 2 : (ja < W.c{2} /\ ! pa r0{1}).
+seq 0 2 : ( ja < W.c{2} /\ ! pa r0{1}).
 wp. call {2} (_: true ==> true). apply A_ll.
 skip. progress. smt.
 while {2} (ja < W.c{2} /\ ! pa r0{1}) (e1{2} + 1 - W.c{2}).
@@ -183,16 +227,19 @@ qed.
 
 
 
-local lemma whp_premat_1 &m pa ia sa ea ra ja : sa <= ja => ja <= ea + 1 =>
-  Pr[ W1.run(pa,ia,sa,ja-1,ra) @ &m : W.c = ja /\ pa res.`2 /\ res.`1 ]
-   =   Pr[ W2.run(pa,ia,sa,ja-1,ea,ra) @ &m : W.c = ja /\ pa res.`2 /\  res.`1 ].
+local lemma whp_premat_1 &m pa ia sa ea ra ja wa : sa <= ja => ja <= ea + 1 =>
+  Pr[ W1(A,D).run((pa,ia,sa,ja-1,ra),wa) @ &m : W.c = ja /\ pa res.`2 /\ res.`1 ]
+   =   Pr[ W2.run((pa,ia,sa,ja-1,ea,ra),wa) @ &m : W.c = ja /\ pa res.`2 /\  res.`1 ].
 proof. move => hp ph.
-byequiv. proc*. inline W1.run. inline W2.run. sp. wp. 
-seq 1 1 : ( ={glob D} /\ ((W.c = ja/\ pa r0 ){1} <=> (W.c = ja/\ pa r0 ){2})  /\  (((W.c = ja/\ pa r0 ){1} /\ (W.c = ja/\ pa r0 ){2})  => ={r0})    ).
-call (whp_premat_1_eq  pa ia sa ea ra ja hp ph). skip. smt.
+byequiv. proc*. inline W1(A,D).run. inline W2.run. sp. wp. 
+seq 1 1 : ( ={w} /\ a0{1}.`2 = a0{2}.`2 /\ ((W.c = ja/\ pa r0 ){1} <=> (W.c = ja/\ pa r0 ){2})  /\  (((W.c = ja/\ pa r0 ){1} /\ (W.c = ja/\ pa r0 ){2})  => ={r0,w0, glob A})    ).
+
+
+call (whp_premat_1_eq  pa ia sa ea ra ja hp ph). skip. progress. smt. smt. smt. smt. smt. smt. smt.
 case (W.c{1} = ja /\ pa r0{1}).
-conseq (_: ={glob W, glob D, r0} ==> _). smt.
-call (_:true). skip. smt. simplify.
+conseq (_: ={glob W, glob A, r0,w0} /\ a0{1}.`2 = a0{2}.`2 ==> _). smt.
+call whp_axp.
+ skip. progress. smt. simplify.
 call {1} (_: true ==> true ).  apply D_ll.
 call {2} (_: true ==> true ).  apply D_ll.
 skip. smt. auto.  auto.
@@ -202,45 +249,52 @@ qed.
 
 
 
-local lemma whp_cap &m p i s ea r ja :  s <= ja => ja <= ea + 1 =>
-   Pr[ W1.run(p,i,s,ea,r) @ &m : W.c = ja /\ p res.`2 /\ res.`1 ]  
-   = Pr[ W1.run(p,i,s,ja-1,r) @ &m : W.c = ja /\ p res.`2 /\ res.`1 ].
+local lemma whp_cap &m p i s ea r ja wa :  s <= ja => ja <= ea + 1 =>
+   Pr[ W1(A,D).run((p,i,s,ea,r),wa) @ &m : W.c = ja /\ p res.`2 /\ res.`1 ]  
+   = Pr[ W1(A,D).run((p,i,s,ja-1,r),wa) @ &m : W.c = ja /\ p res.`2 /\ res.`1 ].
 proof.
 move => sjp jap.
-have ->:  Pr[ W1.run(p,i,s,ja-1,r) @ &m : W.c = ja /\ p res.`2 /\ res.`1 ]
-  =   Pr[ W2.run(p,i,s,ja-1,ea,r) @ &m : W.c = ja /\ p res.`2 /\  res.`1 ].
+have ->:  Pr[ W1(A,D).run((p,i,s,ja-1,r),wa) @ &m : W.c = ja /\ p res.`2 /\ res.`1 ]
+  =   Pr[ W2.run((p,i,s,ja-1,ea,r),wa) @ &m : W.c = ja /\ p res.`2 /\  res.`1 ].
 apply whp_premat_1;auto.
 byequiv (_: a{2} = (p, i, s, ja - 1, ea, r) /\
   (glob D){2} = (glob D){m} /\
   (glob A){2} = (glob A){m} /\
   a{1} = (p, i, s, ea, r) /\
+  w{1} = w{2} /\  
   (glob D){1} = (glob D){m} /\ (glob A){1} = (glob A){m} /\ (glob W){1} = (glob W){2} ==> _).
-proc*. inline W1.run W2.run. wp. sp.
-seq 1 1 : (={glob W, glob D, r0}).
+proc*. inline W1(A,D).run W2.run. wp. sp.
+seq 1 1 : (={glob W, glob A, r0,w0} /\ a0{1}.`2 = a0{2}.`2 ).
 call whp_split_prop.
-skip. progress. smt.
-call (_:true). skip. progress. auto.
-auto.
+skip. progress. smt. smt.
+call whp_axp. skip. progress. smt. auto.
+auto. 
 qed.
 
 
 require import Real.
 
-local lemma whp_cap_fin &m ia (ea : int) r ja   :
+local lemma jjj ia wa &m : 
+   phoare[ W0(A, D).run : arg = (ia,wa) /\ (glob A) = (glob A){m} ==> MyPred res.`2 /\ res.`1 ] =  Pr[W0(A, D).run(ia, wa) @ &m : MyPred res.`2 /\ res.`1] . 
+bypr. progress. rewrite H. simplify. byequiv (_: ={glob A, arg} ==> _).
+proc. call whp_axp. call (_:true). skip. progress. auto. auto.
+qed.
+
+local lemma whp_cap_fin &m ia (ea : int) r ja wa  :
   2  <= ja     =>
   ja <= ea + 1 =>
   MyPred r = false =>
-  (hoare[ A.run : (glob A) = (glob A){m} 
-             ==> (glob A) = (glob A){m} ]) => 
-   Pr[ W1.run(MyPred,ia,1,ea,r) @ &m : W.c = ja /\ MyPred res.`2 /\ res.`1 ]
+   Pr[ W1(A,D).run((MyPred,ia,1,ea,r),wa) @ &m : W.c = ja /\ MyPred res.`2 /\ res.`1 ]
      = (Pr[ A.run(ia) @ &m : !MyPred res ] ^ (ja - 2)) 
-        * Pr[ W0.run(ia) @ &m : MyPred res.`2 /\ res.`1 ]. 
+        * Pr[ W0(A,D).run(ia,wa) @ &m : MyPred res.`2 /\ res.`1 ]. 
 proof. progress.
-have FG :  phoare[ W0.run : arg = ia /\ (glob A) = (glob A){m}  /\ (glob D) = (glob D){m}
-  ==> MyPred res.`2 /\ res.`1 ] = Pr[ W0.run(ia) @ &m : MyPred res.`2 /\ res.`1 ].
+have FG :  phoare[ W0(A,D).run : arg = (ia,wa) /\ (glob A) = (glob A){m}  /\ (glob D) = (glob D){m} 
+  ==> MyPred res.`2 /\ res.`1 ] = Pr[ W0(A,D).run(ia,wa) @ &m : MyPred res.`2 /\ res.`1 ].
 
 bypr. move => &m0 [eq1 eq2].  rewrite eq1. rewrite -eq1.
-byequiv (_: ={glob A, glob D, arg} ==> ={res}).  sim. auto. auto.
+byequiv (_: ={glob A, arg} ==> ={res}).  proc.
+ 
+call whp_axp. call (_:true). skip. progress. smt. smt.
 
 have FF : forall ea, 0 <= ea => phoare[ W(A).whp : 
    arg = (MyPred,ia,1,ea,r) /\ (glob A) = (glob A){m}
@@ -248,39 +302,43 @@ have FF : forall ea, 0 <= ea => phoare[ W(A).whp :
 move => ea0 ea0p.
 
   conseq (final_zz_ph_m A _ _ &m Pr[A.run(ia) @ &m : ! MyPred res]  ia ea0 r _ _ _).  auto. apply A_ll. apply A_rew_ph. auto.  auto. 
-bypr. move => &m0 [eq1 eq2]. rewrite eq1. 
+
+
+
+bypr. move => &m1 [eq1 eq2]. rewrite eq1. 
 byequiv (_: ={arg, glob A} ==> ={res}). sim. progress. rewrite eq2. auto. auto.
-pose p1 := Pr[ W0.run(ia) @ &m : MyPred res.`2 /\ res.`1 ]. auto. auto.
+pose p1 := Pr[ W0(A,D).run(ia,wa) @ &m : MyPred res.`2 /\ res.`1 ].
 rewrite  (whp_cap &m MyPred ia 1 ea r ja ). smt. smt.
-have ->: Pr[W1.run(MyPred, ia, 1, ja - 1, r) @ &m : W.c = ja /\ MyPred res.`2 /\ res.`1]
- = Pr[W3.run(MyPred, ia, 1, ja-1, r) @ &m : W.c = ja /\ MyPred res.`2 /\  res.`1].
-byequiv (_: ={glob W(A), arg, glob D} ==> _). proc*. inline W1.run. 
+have ->: Pr[W1(A,D).run((MyPred, ia, 1, ja - 1, r),wa) @ &m : W.c = ja /\ MyPred res.`2 /\ res.`1]
+ = Pr[W3.run((MyPred, ia, 1, ja-1, r),wa) @ &m : W.c = ja /\ MyPred res.`2 /\  res.`1].
+byequiv (_: ={glob W(A), arg} ==> _). proc*. inline W1(A,D).run. 
 inline W3.run. sp. wp. 
-call (_:true). 
+call whp_axp. 
 call whp_if_prop. skip. progress. 
 auto. auto.
-byphoare (_: arg = (MyPred, ia, 1, ja - 1, r) /\ (glob A) = (glob A){m} ==> _);auto.
-proc. inline W3.M.whp_if. 
-seq 3 : (! p ri) (Pr[ A.run(ia) @ &m : !MyPred res ] ^ (ja - 2))  p1 1%r 0%r (e = ja - 1 /\ W.c <= e  /\ i = ia /\ p = MyPred 
- /\ (!p ri => W.c = e)  /\  (glob A) = (glob A){m} );auto.
-inline W(A).whp. sp.
+
+
+have -> : Pr[W3.run((MyPred, ia, 1, ja - 1, r), wa) @ &m :   W.c = ja /\ MyPred res.`2 /\ res.`1]
+ = Pr[W3'.run((MyPred, ia, 1, ja - 1, r), wa) @ &m :   W.c = ja /\ MyPred res.`2 /\ res.`1].
+byequiv (_: ={glob A, glob W, arg} ==> _). conseq w3w3'.  progress. auto. auto. auto.
+
+byphoare (_: arg = ((MyPred, ia, 1, ja - 1, r),wa) /\ (glob A) = (glob A){m} ==> _);auto.
+proc. inline W3.M.whp_if.  sp.
+seq 1 : (! a.`1 ri) (Pr[ A.run(ia) @ &m : !MyPred res ] ^ (ja - 2))  p1 1%r 0%r (w = wa /\ a.`4 = ja - 1 /\ W.c <= a.`4  /\ a.`2 = ia /\ a.`1 = MyPred 
+ /\ (!a.`1 ri => W.c = a.`4  /\  (glob A) = (glob A){m}) );auto.
+sp. inline W(A).whp. 
 wp.
-while (W.c <= e0 + 1 /\  (glob A) = (glob A){m} ). wp. 
-call H2.
-   skip. progress. smt. skip. progress.   smt. smt.  
+while (W.c <= e + 1 /\ p = MyPred /\ p = MyPred  /\ (!p r0 =>   (glob A) = (glob A){m})). wp. 
+call (A_rew_hoare (glob A){m}).
+   skip. progress. smt. smt.  wp. skip. progress.   smt. smt.  smt.
   call (FF (ja - 2)  ).  smt. wp. skip. progress.  
 rcondt 1. skip. progress. simplify. 
-admit.                          (* TODO: show that p1 = Pr[A @ m] * Pr[D @ m] then  *)
-(* wp. call FG. skip. progress.  *)
-(* smt. *)
-hoare.
-simplify.
-if. wp. call (_:true ==> true). auto.
-wp.  call (_:true ==> true).
-auto. skip. smt.
-call (_: true ==> true). auto. wp. skip.   smt.  
-qed.
 
+call (jjj ia wa &m). sp. skip. progress.  smt. smt.
+
+rcondf 1. skip. progress. smt.
+hoare.  call (_:true).  wp.  skip. progress. smt.
+qed.
 
 require import AllCore Distr FSet StdRing StdOrder StdBigop List.
 (*---*) import RField RealOrder Bigreal BRA.
@@ -289,37 +347,47 @@ require import AllCore Distr FSet StdRing StdOrder StdBigop List.
 
 
 local module CAW = {
-  proc run(a : (rrt -> bool) * irt * int * int * rrt) = {
+  proc run(a : (rrt -> bool) * irt * int * int * rrt,w:de) = {
     var r;
-    r <@ W1.run(a);
+    r <@ W1(A,D).run(a,w);
     return r;
   }
 }.
 
 
-local lemma whp_cap_fin_int_sum_D &m ia pa M (ea : int) ra :
-   Pr[ W1.run(pa,ia,1,ea,ra) @ &m : 1 < W.c <= ea + 1  /\ M res ] = 
+local lemma whp_cap_fin_int_sum_D &m ia pa M (ea : int) ra wa :
+   Pr[ W1(A,D).run((pa,ia,1,ea,ra),wa) @ &m : 1 < W.c <= ea + 1  /\ M res ] = 
     big predT
-      (fun i => Pr[ W1.run(pa,ia,1,ea,ra) @ &m : W.c = i /\ M res ])
+      (fun i => Pr[ W1(A,D).run((pa,ia,1,ea,ra),wa) @ &m : W.c = i /\ M res ])
       (range 2 (ea + 2)).
 progress.
 pose f := fun (x : glob CAW) => x.`1.
-have ->: Pr[ W1.run(pa,ia,1,ea,ra) @ &m : 1 < W.c <= ea + 1 /\ M res ]
-  = Pr[ CAW.run(pa,ia,1,ea,ra) @ &m : 2 <= f (glob CAW) <= ea + 1  /\ M res ].
-byequiv (_: ={arg, glob CAW} ==> ={res, glob CAW}). proc.
+have ->: Pr[ W1(A,D).run((pa,ia,1,ea,ra),wa) @ &m : 1 < W.c <= ea + 1 /\ M res ]
+  = Pr[ CAW.run((pa,ia,1,ea,ra),wa) @ &m : 2 <= f (glob CAW) <= ea + 1  /\ M res ].
+byequiv (_: ={arg, glob A, glob W} ==> ={res, glob W}). proc.
 inline*. sp.  wp. 
 progress.
-sim. auto. smt. 
-rewrite (pr_interval_to_sum_lemma CAW &m (pa, ia, 1, ea, ra) f (fun _ x _ => M x)).
+seq 2 2 : (r{1} = r0{2} /\ w{1} = w0{2} /\ a{1}.`2 = a0{2}.`2 /\ ={glob A, glob W}). sim.
+
+call whp_axp. skip. progress.  smt. auto. 
+smt.
+
+
+rewrite (pr_interval_to_sum_lemma CAW &m ((pa, ia, 1, ea, ra),wa) f (fun _ x _ => M x)).
 simplify.
-have <-:  (fun (i : int) => Pr[W1.run(pa, ia, 1, ea, ra) @ &m : W.c = i /\ M res])
+have <-:  (fun (i : int) => Pr[W1(A,D).run((pa, ia, 1, ea, ra),wa) @ &m : W.c = i /\ M res])
  = (fun (i : int) =>
-     Pr[CAW.run(pa, ia, 1, ea, ra) @ &m : f ( (glob CAW)) = i /\ M res]).
+     Pr[CAW.run((pa, ia, 1, ea, ra),wa) @ &m : f ( (glob CAW)) = i /\ M res]).
 apply fun_ext. move => x.
-byequiv (_: ={arg, glob CAW} ==> ={res, glob CAW}). proc.
+byequiv (_: ={arg, glob A, glob W} ==> ={res, glob W}). proc.
 inline*.  wp.  sp.
-sim. auto. smt. 
-auto.
+seq 2 2 : (r{1} = r0{2} /\ w{1} = w0{2} /\ a{1}.`2 = a0{2}.`2 /\ ={glob A, glob W}). sim.
+
+call whp_axp. skip. progress.  smt. auto. 
+smt.
+
+
+ auto. 
 qed.
 
 
@@ -344,37 +412,35 @@ wp. call (_: true ==> true). auto. skip. auto. auto.
 qed.
 
 
-local lemma whp_cap_fin_int_D &m pa ia (ea : int) ra :
+local lemma whp_cap_fin_int_D &m pa ia (ea : int) ra wa:
   pa ra = false => 1 <= ea =>
-   Pr[ W1.run(pa,ia,1,ea,ra) @ &m : 1 < W.c <= ea + 1 ] = 1%r.
-progress. byphoare (_: arg = (pa, ia, 1, ea, ra) ==> _).
+   Pr[ W1(A,D).run((pa,ia,1,ea,ra),wa) @ &m : 1 < W.c <= ea + 1 ] = 1%r.
+progress. byphoare (_: arg = ((pa, ia, 1, ea, ra),wa) ==> _).
 proc.  call (_:true ==> true). apply D_ll. 
 call (whp_cap_fin_int pa ia ea ra). skip. auto. auto. auto.
 qed.
 
 
-local lemma whp_cap_fin_sum' &m  ia (ea : int) r :
+local lemma whp_cap_fin_sum' &m  ia (ea : int) r wa :
   MyPred r = false =>
   1 <= ea =>
-  hoare[ A.run : (glob A) = (glob A){m} 
-           ==> (glob A) = (glob A){m} ] => 
-  Pr[ W1.run(MyPred,ia,1,ea,r) @ &m : MyPred res.`2 /\ res.`1 ]  
+  Pr[ W1(A,D).run((MyPred,ia,1,ea,r),wa) @ &m : MyPred res.`2 /\ res.`1 ]  
      = big predT
         (fun i => (Pr[ A.run(ia) @ &m : !MyPred res ] ^ (i - 2)) 
-          * Pr[ W0.run(ia) @ &m : MyPred res.`2 /\ res.`1 ]  )
+          * Pr[ W0(A,D).run(ia,wa) @ &m : MyPred res.`2 /\ res.`1 ]  )
         (range 2 (ea + 2)). 
 proof. progress.
-have ->: Pr[ W1.run(MyPred,ia,1,ea,r) @ &m : MyPred res.`2 /\ res.`1 ]  
- = Pr[ W1.run(MyPred,ia,1,ea,r) @ &m : (1 < W.c <= ea + 1) 
+have ->: Pr[ W1(A,D).run((MyPred,ia,1,ea,r),wa) @ &m : MyPred res.`2 /\ res.`1 ]  
+ = Pr[ W1(A,D).run((MyPred,ia,1,ea,r),wa) @ &m : (1 < W.c <= ea + 1) 
         /\ MyPred res.`2 /\ res.`1 ].
 rewrite Pr[mu_split (1 < W.c && W.c <= ea + 1)].
-  have ->: Pr[W1.run(MyPred, ia, 1, ea, r) @ &m :
+  have ->: Pr[W1(A,D).run((MyPred, ia, 1, ea, r),wa) @ &m :
    (MyPred res.`2 /\ res.`1) /\ ! (1 < W.c && W.c <= ea + 1)] = 0%r.
-   have : Pr[W1.run(MyPred, ia, 1, ea, r) @ &m : ! (1 < W.c && W.c <= ea + 1)] = 0%r.
-    have f3 : Pr[W1.run(MyPred, ia, 1, ea, r) @ &m : (1 < W.c && W.c <= ea + 1)] = 1%r. rewrite (whp_cap_fin_int_D &m). smt.
+   have : Pr[W1(A,D).run((MyPred, ia, 1, ea, r),wa) @ &m : ! (1 < W.c && W.c <= ea + 1)] = 0%r.
+    have f3 : Pr[W1(A,D).run((MyPred, ia, 1, ea, r),wa) @ &m : (1 < W.c && W.c <= ea + 1)] = 1%r. rewrite (whp_cap_fin_int_D &m). smt.
   smt. 
-    have f2 : 1%r = Pr[W1.run(MyPred, ia, 1, ea, r) @ &m : ! (1 < W.c && W.c <= ea + 1)] + Pr[W1.run(MyPred, ia, 1, ea, r) @ &m : (1 < W.c && W.c <= ea + 1)]. 
-    have  <- : Pr[W1.run(MyPred, ia, 1, ea, r) @ &m : true ] = 1%r.
+    have f2 : 1%r = Pr[W1(A,D).run((MyPred, ia, 1, ea, r),wa) @ &m : ! (1 < W.c && W.c <= ea + 1)] + Pr[W1(A,D).run((MyPred, ia, 1, ea, r),wa) @ &m : (1 < W.c && W.c <= ea + 1)]. 
+    have  <- : Pr[W1(A,D).run((MyPred, ia, 1, ea, r),wa) @ &m : true ] = 1%r.
     smt.
    rewrite Pr[mu_split (1 < W.c && W.c <= ea + 1)]. simplify.
    smt. auto. timeout 20. smt. smt. smt.
@@ -387,35 +453,30 @@ progress.
 rewrite (whp_cap_fin &m).  auto. smt.
 auto.
 auto.
-auto.
 qed.
 
 
-local lemma whp_cap_fin_sum'' &m  ia (ea : int) r :
+local lemma whp_cap_fin_sum'' &m  ia (ea : int) r wa:
   MyPred r = false =>
   1 <= ea =>
-  hoare[ A.run : (glob A) = (glob A){m} 
-           ==> (glob A) = (glob A){m} ] => 
-   Pr[ W1.run(MyPred,ia,1,ea,r) @ &m : MyPred res.`2 /\ res.`1 ]  
+   Pr[ W1(A,D).run((MyPred,ia,1,ea,r),wa) @ &m : MyPred res.`2 /\ res.`1 ]  
       = big predT
          (fun i => (Pr[ A.run(ia) @ &m : !MyPred res ] ^ i) 
-           * Pr[ W0.run(ia) @ &m : MyPred res.`2 /\ res.`1 ])
+           * Pr[ W0(A,D).run(ia,wa) @ &m : MyPred res.`2 /\ res.`1 ])
          (range 0 ea). 
 proof. progress.
 rewrite (whp_cap_fin_sum' &m);auto.
 rewrite (PIT.big_reindex (fun (i : int) =>
-     Pr[A.run(ia) @ &m : ! MyPred res] ^ i * Pr[W0.run(ia) @ &m : MyPred res.`2 /\  res.`1]) 2 ea). auto.
+     Pr[A.run(ia) @ &m : ! MyPred res] ^ i * Pr[W0(A,D).run(ia,wa) @ &m : MyPred res.`2 /\  res.`1]) 2 ea). auto.
 qed.
 
 
-local lemma whp_cap_fin_sum &m ia (ea : int) r :
+lemma whp_cap_fin_sum &m ia (ea : int) r wa :
   MyPred r = false =>
-  hoare[ A.run : (glob A) = (glob A){m} 
-           ==> (glob A) = (glob A){m} ] => 
-  Pr[ W1.run(MyPred,ia,1,ea,r) @ &m : MyPred res.`2 /\ res.`1 ]  
+  Pr[ W1(A,D).run((MyPred,ia,1,ea,r),wa) @ &m : MyPred res.`2 /\ res.`1 ]  
      = big predT
         (fun i => (Pr[ A.run(ia) @ &m : !MyPred res ] ^ i) 
-          * Pr[ W0.run(ia) @ &m : MyPred res.`2 /\ res.`1 ])
+          * Pr[ W0(A,D).run(ia,wa) @ &m : MyPred res.`2 /\ res.`1 ])
         (range 0 ea). 
 proof.
 case (1 <= ea).
@@ -423,13 +484,13 @@ progress. rewrite (whp_cap_fin_sum'' &m);auto.
 progress.
 have ->: bigi predT
   (fun (i : int) =>
-     Pr[A.run(ia) @ &m : ! MyPred res] ^ i * Pr[W0.run(ia) @ &m : MyPred res.`2 /\ res.`1])
+     Pr[A.run(ia) @ &m : ! MyPred res] ^ i * Pr[W0(A,D).run(ia,wa) @ &m : MyPred res.`2 /\ res.`1])
   0 ea = 0%r.
 smt.
-byphoare (_: arg = (MyPred, ia, 1, ea, r) ==> _).
+byphoare (_: arg = ((MyPred, ia, 1, ea, r),wa) ==> _).
 hoare.
 conseq (_: _ ==> ! MyPred res.`2). smt.
-proc. sp. simplify. inline W1.M.whp. sp.
+proc. sp. simplify. inline W1(A,D).M.whp. sp.
 rcondf 1. skip. smt. call (_: true ==> true). auto. wp. skip. smt. auto. auto.
 qed.
 
